nola/iris/store.v
@@ -1,155 +1,46 @@
 (** * Stored propositions *)
 
 From nola.bi Require Export internal modw.
-From nola.iris Require Export iprop.
-From nola.iris Require Import sinv.
-From iris.base_logic Require Import lib.token.
+From nola.iris Require Export cif dinv.
+From iris.base_logic Require Export lib.token.
 From iris.proofmode Require Import proofmode.
-Import iPropAppNotation ModwNotation.
+Import iPropAppNotation ModwNotation DsemNotation.
 
-Implicit Type (FML : oFunctor) (i : positive).
-
-(** Formula for stored propositions *)
-Local Definition store_fml FML : oFunctor := boolO * FML.
-
-(** Formula for stored propositions *)
-Class storeGpreS FML Σ := StoreGpreS {
-  storeGpreS_sinv : sinvGpreS (store_fml FML) Σ;
-  storeGpreS_token : tokenG Σ;
-}.
-Local Existing Instance storeGpreS_sinv.
-Local Existing Instance storeGpreS_token.
-Class storeGS FML Σ := StoreGS {
-  storeGS_sinv : sinvGS (store_fml FML) Σ;
-  storeGS_token : tokenG Σ;
-}.
-Local Existing Instance storeGS_sinv. Local Existing Instance storeGS_token.
-Definition storeΣ FML `{!oFunctorContractive FML} :=
-  #[sinvΣ (store_fml FML); tokenΣ].
-#[export] Instance subG_storeΣ
-  `{!oFunctorContractive FML, !subG (storeΣ FML) Σ} : storeGpreS FML Σ.
-Proof. solve_inG. Qed.
+Implicit Type FML : oFunctor.
 
 Section store.
-  Context `{!storeGS FML Σ}.
-  Implicit Type (Px : FML $oi Σ) (bPx : store_fml FML $oi Σ).
+  Context `{!dinvGS (cifOF CON) Σ, tokenG Σ, !Csem CON JUDG Σ}.
+  Implicit Type Px : cif CON Σ.
 
   (** [store_tok]: Exclusive stored proposition token *)
-  Local Definition store_tok_def (Px : FML $oi Σ) : iProp Σ :=
-    ∃ i, token i ∗ sinv_tok i (true, Px).
+  Local Definition store_tok_def Px : iProp Σ :=
+    ∃ γ, token γ ∗ dinv_tok (Px ∨ ▷ token γ)%cif.
   Local Definition store_tok_aux : seal store_tok_def. Proof. by eexists. Qed.
   Definition store_tok := store_tok_aux.(unseal).
   Local Lemma store_tok_unseal : store_tok = store_tok_def.
   Proof. exact: seal_eq. Qed.
 
-  (** [pstore_tok]: Persistent stored proposition token *)
-  Local Definition pstore_tok_def (Px : FML $oi Σ) : iProp Σ :=
-    ∃ i, sinv_tok i (false, Px).
-  Local Definition pstore_tok_aux : seal pstore_tok_def. Proof. by eexists. Qed.
-  Definition pstore_tok := pstore_tok_aux.(unseal).
-  Local Lemma pstore_tok_unseal : pstore_tok = pstore_tok_def.
-  Proof. exact: seal_eq. Qed.
-
-  (** [store_tok] and [pstore_tok] are non-expansive *)
+  (** [store_tok] is non-expansive *)
   #[export] Instance store_tok_ne : NonExpansive store_tok.
   Proof. rewrite store_tok_unseal. solve_proper. Qed.
   #[export] Instance store_tok_proper : Proper ((≡) ==> (⊣⊢)) store_tok.
   Proof. apply ne_proper, _. Qed.
-  #[export] Instance pstore_tok_ne : NonExpansive pstore_tok.
-  Proof. rewrite pstore_tok_unseal. solve_proper. Qed.
-  #[export] Instance pstore_tok_proper : Proper ((≡) ==> (⊣⊢)) pstore_tok.
-  Proof. apply ne_proper, _. Qed.
-  (** [pstore_tok] is persistent *)
-  #[export] Instance pstore_tok_persistent {Px} : Persistent (pstore_tok Px).
-  Proof. rewrite pstore_tok_unseal. exact _. Qed.
-  (** [store_tok] and [pstore_tok] are timeless for discrete formulas *)
-  #[export] Instance store_tok_timeless `{!Discrete Px} :
-    Timeless (store_tok Px).
-  Proof. rewrite store_tok_unseal. exact _. Qed.
-  #[export] Instance pstore_tok_timeless `{!Discrete Px} :
-    Timeless (pstore_tok Px).
-  Proof. rewrite pstore_tok_unseal. exact _. Qed.
-
-  (** Semantics *)
-  Local Definition store_sem (sm : FML $oi Σ → iProp Σ) i bPx : iProp Σ :=
-    (if bPx.1 then sm bPx.2 ∨ token i else □ sm bPx.2)%I.
-  Arguments store_sem _ _ _ /.
-  (** [store_sem sm] is non-expansive when [sm] is *)
-  Local Lemma store_sem_ne {sm} :
-    internal_ne sm ⊢@{iProp Σ} ∀ i, internal_ne (store_sem sm i).
-  Proof.
-    iIntros "#Ne" (?[b ?][??]). rewrite prod_equivI /= discrete_eq.
-    rewrite leibniz_equiv_iff. iIntros "[%eq ≡]". move: eq=> <-.
-    case: b; by iRewrite ("Ne" with "≡").
-  Qed.
-
-  (** World satisfaction *)
-  Local Definition store_wsat_def (sm : FML $oi Σ -d> iProp Σ) : iProp Σ :=
-    sinv_wsat (store_sem sm).
-  Local Definition store_wsat_aux : seal store_wsat_def. Proof. by eexists. Qed.
-  Definition store_wsat := store_wsat_aux.(unseal).
-  Local Lemma store_wsat_unseal : store_wsat = store_wsat_def.
-  Proof. exact: seal_eq. Qed.
-
-  (** [store_wsat] is non-expansive *)
-  #[export] Instance store_wsat_ne : NonExpansive store_wsat.
-  Proof.
-    rewrite store_wsat_unseal. unfold store_wsat_def, store_sem. solve_proper.
-  Qed.
-  #[export] Instance store_wsat_proper : Proper ((≡) ==> (≡)) store_wsat.
-  Proof. apply ne_proper, _. Qed.
 
   (** Allocate [store_tok] *)
-  Lemma store_tok_alloc {sm} Px : sm Px =[store_wsat sm]=∗ store_tok Px.
+  Lemma store_tok_alloc {δ} Px : ⟦ Px ⟧(δ) =[dinv_wsat ⟦⟧(δ)]=∗ store_tok Px.
   Proof.
-    rewrite store_tok_unseal store_wsat_unseal. iIntros "Px W".
-    iDestruct (sinv_tok_alloc_suspend (FML:=store_fml _) (true, Px) with "W")
-      as (I) "big".
-    iMod (token_alloc_strong (.∉ I)) as (??) "$".
-    { apply (pred_infinite_set (C:=gset positive))=> X. exists (fresh (I ∪ X)).
-      apply not_elem_of_union, is_fresh. }
-    iMod ("big" with "[//]") as "[$ →W]". iModIntro. iApply "→W". by iLeft.
-  Qed.
-
-  (** Allocate [pstore_tok] suspending the world satisfaction *)
-  Lemma pstore_tok_alloc_suspend {sm} Px :
-    store_wsat sm ==∗ pstore_tok Px ∗ (□ sm Px -∗ store_wsat sm).
-  Proof.
-    rewrite pstore_tok_unseal store_wsat_unseal. iIntros "W".
-    iDestruct (sinv_tok_alloc_suspend (FML:=store_fml _) (false, Px) with "W")
-      as (I) "big".
-    iMod ("big" $! (fresh I) with "[%]") as "[#inv →W]". { apply is_fresh. }
-    iModIntro. iFrame "inv". iIntros "?". by iApply "→W".
-  Qed.
-  (** Allocate [pstore_tok] *)
-  Lemma pstore_tok_alloc {sm} Px : □ sm Px =[store_wsat sm]=∗ pstore_tok Px.
-  Proof.
-    iIntros "? W". iMod (pstore_tok_alloc_suspend with "W") as "[$ →W]".
-    iModIntro. by iApply "→W".
+    rewrite store_tok_unseal. iIntros "Px W". iMod token_alloc as (γ) "$".
+    iMod (dinv_tok_alloc_suspend (FML:=cifOF _) (Px ∨ ▷ token γ)%cif
+      with "W") as "/=[$ cl]".
+    iModIntro. iApply "cl". iFrame.
   Qed.
 
   (** Access the content of [store_tok] *)
-  Lemma store_tok_acc {sm} Px : store_tok Px -∗[store_wsat sm] sm Px.
+  Lemma store_tok_acc {δ} Px : store_tok Px -∗[dinv_wsat ⟦⟧(δ)]◇ ⟦ Px ⟧(δ).
   Proof.
-    rewrite store_tok_unseal store_wsat_unseal. iIntros "[%[tok inv]] W".
-    iDestruct (sinv_tok_acc with "inv W") as "/=[[$|tok'] →W]"; last first.
-    { iDestruct (token_exclusive with "tok tok'") as %[]. }
-    iApply "→W". by iRight.
-  Qed.
-  (** Access the content of [pstore_tok] *)
-  Lemma pstore_tok_acc {sm} Px : pstore_tok Px -∗[store_wsat sm] □ sm Px.
-  Proof.
-    rewrite pstore_tok_unseal store_wsat_unseal. iIntros "[% inv] W".
-    iDestruct (sinv_tok_acc with "inv W") as "/=[#Px →W]". iFrame "Px".
-    by iApply "→W".
+    rewrite store_tok_unseal. iIntros "[%[t i]] W".
+    iDestruct (dinv_tok_acc with "i W") as "/=[[$|>t'] →W]"; last first.
+    { iDestruct (token_exclusive with "t t'") as %[]. }
+    iModIntro. iApply "→W". by iRight.
   Qed.
 End store.
-
-(** Allocate [store_wsat] *)
-Lemma store_wsat_alloc `{!storeGpreS FML Σ} :
-  ⊢ |==> ∃ _ : storeGS FML Σ, ∀ sm, internal_ne sm -∗ store_wsat sm.
-Proof.
-  iMod sinv_wsat_alloc as (γ) "W". iModIntro. iExists (StoreGS _ _ _ _).
-  iIntros (?) "Ne". rewrite store_wsat_unseal. iApply "W".
-  by iApply store_sem_ne.
-Qed.
